%\begin{frame}
%\frametitle{Overskrift}
%\begin{itemize}
%\item Fisk
%\end{itemize}
%\end{frame}
%
% JULIE
\subsection{Runge-Kutta metoder}
\begin{frame}
\frametitle{Eulers metode } 
\begin{minipage}[b]{0.31\textwidth}
\begin{align*}
x_{n+1} & = x_n+h \\
y_{n+1} & = y_n + h f(x_n,y_n) \\
\phantom{x_1}\\
\\
\\
\end{align*}
\end{minipage}
\phantom{hejmeddig}
%
\input{images/euler}
\\
\phantom{H}
\\
%
\end{frame}
%
%
%
%
\begin{frame}
\frametitle{Korrigeret Eulersmetode $\alpha = \frac{1}{2}$ } 
\begin{minipage}[t]{0.31\textwidth}
\begin{align*}
k_1 & = f(x_n , y_n) \\
k_2 & = f \left( x_n + \frac{h}{2} , y_n + \frac{h}{2} k_1 \right)  \\
\end{align*}
\end{minipage} 
\phantom{Hej}
\begin{minipage}[t]{0.31\textwidth}
\begin{align*}
x_{n+1} & = x_n+h \\
y_{n+1} & = y_n + h k_2 \\
\end{align*}
\end{minipage} 
\\
%
\input{images/korri}
\\
\phantom{H}
\\
%
\end{frame}
%
%
%
\begin{frame}
\frametitle{Modificeret Eulersmetode $\alpha = 1$}  
\begin{minipage}[t]{0.31\textwidth}
\begin{align*}
k_1 & = f(x_n , y_n) \\
k_2 & = f( x_n + h , y_n  + h k_1 ) \\
\end{align*}
%
\end{minipage} 
\phantom{Hej}
\begin{minipage}[t]{0.31\textwidth}
\begin{align*}
x_{n+1} & = x_n+h \\
y_{n+1} & = y_n + \frac{h}{2} (k_1 + k_2 ) \\
\end{align*}
%
\end{minipage} 
\\
\input{images/modi}
\\
\phantom{H}
\\
%
\end{frame}
%
%
% MADS
\begin{frame}
\frametitle{Heuns metode $\alpha = \frac{2}{3}$ }
\begin{minipage}[t]{0.31\textwidth}
\begin{align*}
k_1 & = f(x_n , y_n) \\
k_2 & = f \left( x_n + \frac{2}{3} h , y_n  + \frac{2}{3} h k_1 \right) \\
\end{align*}
%
\end{minipage} 
\phantom{Hej}
\begin{minipage}[t]{0.31\textwidth}
\begin{align*}
x_{n+1} & = x_n+h \\
y_{n+1} & = y_n + \frac{h}{4} (k_1 + 3k_2 )  \\
\end{align*}
%
\end{minipage} 
\\
\input{images/heun}
\\
\phantom{H}
\\
\end{frame}