\section*{2.}
%
\begin{align}
f(\frac{L}{2})	&= h_0 + \lambda cosh (\frac{L}{2 \lambda}) = h\\
f(0)			&= h_0 + \lambda = h-s
\end{align}
%
Disse $2$ ligninger kan give anledning til en ny ligning.
%
\begin{align}
h_0 + \lambda \cosh (\frac{L}{2 \lambda}) -(h_0 + \lambda \cosh (\frac{L}{2 \lambda})) &= h_0 + \lambda -(h_0 + \lambda)\\
h_0 + \lambda \cosh (\frac{L}{2 \lambda}) - h &= h_0 + \lambda - (h - s)\\
\lambda \cosh (\frac{L}{2 \lambda}) - h &= \lambda - h + s\\
\lambda \cosh (\frac{L}{2 \lambda}) &= \lambda + s
\end{align}